Simplify use of term tuples.

lib.v
@@ -1,5 +1,5 @@
 From stdpp Require Import base countable gmap.
-From iris.heap_lang Require Import lang notation.
+From iris.heap_lang Require Import lang notation proofmode.
 
 Definition perm `{!EqDecision T, !Countable T} (X : gset (T * T)) :=
   forall p1 p2, p1 ∈ X → p2 ∈ X → (p1.1 = p2.1 ↔ p1.2 = p2.2).
@@ -7,10 +7,27 @@ Definition perm `{!EqDecision T, !Countable T} (X : gset (T * T)) :=
 Definition flipb {T S} (b : bool) (f : T → T → S) x y :=
   f (if b then x else y) (if b then y else x).
 
-Class AsVal A := as_val : A -> val.
+Class Repr A := repr : A -> val.
 
-Instance as_val_option `{AsVal A} : AsVal (option A) := λ x,
+Instance repr_option `{Repr A} : Repr (option A) := λ x,
   match x with
-  | Some x => SOMEV (as_val x)
+  | Some x => SOMEV (repr x)
   | None => NONEV
   end.
+
+Instance repr_list `{Repr A} : Repr (list A) :=
+  fold_right (fun x v => (repr x, v)%V) #0.
+
+Definition get_list : val := rec: "loop" "l" "n" :=
+  if: "l" = #0 then NONE
+  else if: "n" = #0 then SOME (Fst "l")
+  else "loop" (Snd "l") ("n" - #1).
+
+Lemma twp_get_list `{!Repr A, !heapG Σ} (l : list A) (n : nat) :
+  ⊢ WP get_list (repr l) #n
+       [{v, ⌜v = repr (nth_error l n)⌝}].
+Proof.
+rewrite /repr; elim: n l=> [|n IH] [|x l] /=; wp_rec; wp_pures; eauto.
+rewrite (_ : (S n - 1)%Z = n); try lia.
+by iApply IH.
+Qed.
